ictr irmin example modified

irmin-example/ictr/out/Ictr.ml
@@ -1,55 +1,86 @@
 (* open Prims *)
 type s = int
 type t = int [@@deriving irmin]
+type rval =
+  | Val of s 
+  | Bot 
+let (uu___is_Val : rval -> bool) =
+  fun projectee -> match projectee with | Val _0 -> true | uu___ -> false
+let (__proj__Val__item___0 : rval -> s) =
+  fun projectee -> match projectee with | Val _0 -> _0
+let (uu___is_Bot : rval -> bool) =
+  fun projectee -> match projectee with | Bot -> true | uu___ -> false
 type op =
   | Add 
-let (uu___is_Add : op -> bool) = fun projectee -> true
+  | Rd 
+let (uu___is_Add : op -> bool) =
+  fun projectee -> match projectee with | Add -> true | uu___ -> false
+let (uu___is_Rd : op -> bool) =
+  fun projectee -> match projectee with | Rd -> true | uu___ -> false
 let (init : int) = 0
-let pre_cond_op : 'uuuuu 'uuuuu1 . 'uuuuu -> 'uuuuu1 -> bool =
+let pre_cond_do : 'uuuuu 'uuuuu1 . 'uuuuu -> 'uuuuu1 -> bool =
   fun s1 -> fun op1 -> true
-let (app_op : s -> (int * op) -> s) =
-  fun s1 -> fun op1 -> match op1 with | (uu___, Add) -> s1 + 1
+let pre_cond_prop_do :
+  'uuuuu 'uuuuu1 'uuuuu2 . 'uuuuu -> 'uuuuu1 -> 'uuuuu2 -> bool =
+  fun tr -> fun s1 -> fun op1 -> true
+let (do1 : s -> (int * op) -> (s * rval)) =
+  fun s1 ->
+    fun op1 ->
+      match op1 with
+      | (uu___, Add) -> ((s1 + 1), Bot)
+      | (uu___, Rd) -> (s1, (Val s1))
 let rec (sum : (int * op) list -> int) =
   fun l ->
     match l with
     | [] -> 0
     | (uu___, Add)::xs -> (sum xs) + 1
+    | (uu___, Rd)::xs -> sum xs
+let (spec : (int * op) -> op Library.ae -> rval) =
+  fun o ->
+    fun tr ->
+      match o with
+      | (uu___, Add) -> Bot
+      | (uu___, Rd) -> Val (sum (Library.__proj__A__item__l tr))
 let (sim : op Library.ae -> s -> bool) =
   fun tr -> fun s1 -> s1 = (sum (Library.__proj__A__item__l tr))
 
-let (pre_cond_merge1 : int -> int -> int -> bool) =
+
+let (pre_cond_merge : int -> int -> int -> bool) =
   fun l -> fun a -> fun b -> (a >= l) && (b >= l)
-let (merge1 : s -> s -> s -> s) = fun l -> fun a -> fun b -> (a + b) - l
-let pre_cond_merge :
+let pre_cond_prop_merge :
   'uuuuu 'uuuuu1 'uuuuu2 'uuuuu3 'uuuuu4 'uuuuu5 .
     'uuuuu ->
       'uuuuu1 -> 'uuuuu2 -> 'uuuuu3 -> 'uuuuu4 -> 'uuuuu5 -> bool
   = fun ltr -> fun l -> fun atr -> fun a -> fun btr -> fun b -> true
-let (merge :
-  op Library.ae -> s -> op Library.ae -> s -> op Library.ae -> s -> s) =
-  fun ltr -> fun l -> fun atr -> fun a -> fun btr -> fun b -> merge1 l a b
+let (merge : s -> s -> s -> s) = fun l -> fun a -> fun b -> (a + b) - l
 
-let (uu___173 : (s, op) Library.mrdt) =
+
+
+
+
+let (ictr : (s, op, rval) Library.mrdt) =
   {
     Library.init = init;
-    Library.pre_cond_op = pre_cond_op;
-    Library.app_op = app_op;
+    Library.spec = spec;
     Library.sim = sim;
+    Library.pre_cond_do = pre_cond_do;
+    Library.pre_cond_prop_do = pre_cond_prop_do;
     Library.pre_cond_merge = pre_cond_merge;
-    Library.pre_cond_merge1 = pre_cond_merge1;
-    Library.merge1 = merge1;
+    Library.pre_cond_prop_merge = pre_cond_prop_merge;
+    Library.do1 = do1;
     Library.merge = merge;
+    Library.prop_do = ();
     Library.prop_merge = ();
-    Library.prop_oper = ();
+    Library.prop_spec = ();
     Library.convergence = ()
   }
+
+
 
 let merge ~old a b =
 	let open Irmin.Merge.Infix in
 	old () >>=* fun old ->
-  let _old = (match old with None -> 0 | Some l -> l) in
-  Irmin.Merge.ok (merge1 _old a b)
+ let _old = (match old with None -> 0 | Some l -> Printf.printf "Merge called %d %d %d\n" l a b;  l) in
+  Irmin.Merge.ok (merge _old a b)
 
 let merge = Irmin.Merge.(option (v t merge))
-
-
